VCVio/OracleComp/DistSemantics/List.lean
@@ -103,7 +103,7 @@ end append
 section mapM
 
 @[simp]
-lemma probFailure_list_mapM_loop [spec.FiniteRange]
+lemma probFailure_list_mapM_loop {α β : Type*} [spec.FiniteRange]
     (xs : List α) (f : α → OracleComp spec β) (ys : List β) :
     [⊥ | List.mapM.loop f xs ys] = 1 - (xs.map (1 - [⊥ | f ·])).prod := by
   revert ys
@@ -123,12 +123,12 @@ lemma probFailure_list_mapM_loop [spec.FiniteRange]
   }
 
 @[simp]
-lemma probFailure_list_mapM [spec.FiniteRange] (xs : List α) (f : α → OracleComp spec β) :
+lemma probFailure_list_mapM {α β : Type*} [spec.FiniteRange] (xs : List α) (f : α → OracleComp spec β) :
     [⊥ | xs.mapM f] = 1 - (xs.map (1 - [⊥ | f ·])).prod := by
   rw [mapM, probFailure_list_mapM_loop]
 
 @[simp]
-lemma probOutput_list_mapM_loop [DecidableEq β] [spec.FiniteRange]
+lemma probOutput_list_mapM_loop {α β : Type*} [DecidableEq β] [spec.FiniteRange]
     (xs : List α) (f : α → OracleComp spec β) (ys : List β)
     (zs : List β) : [= zs | List.mapM.loop f xs ys] =
       if zs.length = xs.length + ys.length ∧ zs.take ys.length = ys.reverse
@@ -168,7 +168,7 @@ lemma probOutput_list_mapM_loop [DecidableEq β] [spec.FiniteRange]
   · simp [h]
 
 @[simp]
-lemma probOutput_list_mapM [spec.FiniteRange] (xs : List α) (f : α → OracleComp spec β)
+lemma probOutput_list_mapM {α β : Type*} [spec.FiniteRange] (xs : List α) (f : α → OracleComp spec β)
     (ys : List β) : [= ys | xs.mapM f] = if ys.length = xs.length
       then (List.zipWith (λ x y ↦ [= y | f x]) xs ys).prod else 0 := by
   have : DecidableEq β := Classical.decEq β; simp [List.mapM]
